Transition.thy
@@ -1,7 +1,7 @@
 section\<open>Transitions\<close>
-text\<open>Here we define the 'a transitions which make up EFSMs. As per \cite{foster2018}, each 'a transition
+text\<open>Here we define the transitions which make up EFSMs. As per \cite{foster2018}, each transition
 has a label and an arity and, optionally, guards, outputs, and updates. To implement this, we use
-the record type such that each component of the 'a transition can be accessed.\<close>
+the record type such that each component of the transition can be accessed.\<close>
 
 theory Transition
 imports GExp
@@ -9,63 +9,61 @@ begin
 
 type_synonym label = String.literal
 type_synonym arity = nat
-type_synonym 'a guard = "(vname, 'a) gexp"
-type_synonym 'a inputs = "'a list"
-type_synonym 'a outputs = "'a option list"
-type_synonym 'a output_function = "(vname, 'a) aexp"
-type_synonym 'a update_function = "nat \<times> (vname, 'a) aexp"
-type_synonym 'b datastate = "vname \<Rightarrow> 'b option"
+type_synonym guard = "vname gexp"
+type_synonym inputs = "value list"
+type_synonym outputs = "value option list"
+type_synonym output_function = "vname aexp"
+type_synonym update_function = "nat \<times> vname aexp"
 
-
-text_raw\<open>\snip{'a transitiontype}{1}{2}{%\<close>
-record 'a transition =
+text_raw\<open>\snip{transitiontype}{1}{2}{%\<close>
+record transition =
   Label :: String.literal
   Arity :: nat
-  Guards :: "'a guard list"
-  Outputs :: "'a output_function list"
-  Updates :: "'a update_function list"
+  Guards :: "guard list"
+  Outputs :: "output_function list"
+  Updates :: "update_function list"
 text_raw\<open>}%endsnip\<close>
 
-definition same_structure :: "'a transition \<Rightarrow> 'a transition \<Rightarrow> bool" where
+definition same_structure :: "transition \<Rightarrow> transition \<Rightarrow> bool" where
   "same_structure t1 t2 = (
     Label t1 = Label t2 \<and>
     Arity t1 = Arity t2 \<and>
     length (Outputs t1) = length (Outputs t2)
   )"
 
-definition enumerate_inputs :: "'a transition \<Rightarrow> nat set" where
+definition enumerate_inputs :: "transition \<Rightarrow> nat set" where
   "enumerate_inputs t = (\<Union> (set (map enumerate_gexp_inputs (Guards t)))) \<union>
                         (\<Union> (set (map enumerate_aexp_inputs (Outputs t)))) \<union>
                         (\<Union> (set (map (\<lambda>(_, u). enumerate_aexp_inputs u) (Updates t))))"
 
-definition max_input :: "'a transition \<Rightarrow> nat option" where
+definition max_input :: "transition \<Rightarrow> nat option" where
   "max_input t = (if enumerate_inputs t = {} then None else Some (Max (enumerate_inputs t)))"
 
-definition total_max_input :: "'a transition \<Rightarrow> nat" where
+definition total_max_input :: "transition \<Rightarrow> nat" where
   "total_max_input t = (case max_input t of None \<Rightarrow> 0 | Some a \<Rightarrow> a)"
 
-definition enumerate_regs :: "'a transition \<Rightarrow> nat set" where
+definition enumerate_regs :: "transition \<Rightarrow> nat set" where
   "enumerate_regs t = (\<Union> (set (map GExp.enumerate_regs (Guards t)))) \<union>
                       (\<Union> (set (map AExp.enumerate_regs (Outputs t)))) \<union>
                       (\<Union> (set (map (\<lambda>(_, u). AExp.enumerate_regs u) (Updates t)))) \<union>
-                      (\<Union> (set (map (\<lambda>(r, _). {r}) (Updates t))))"
+                      (\<Union> (set (map (\<lambda>(r, _). AExp.enumerate_regs (V (R r))) (Updates t))))"
 
-definition max_reg :: "'a transition \<Rightarrow> nat option" where
+definition max_reg :: "transition \<Rightarrow> nat option" where
   "max_reg t = (if enumerate_regs t = {} then None else Some (Max (enumerate_regs t)))"
 
-definition total_max_reg :: "'a transition \<Rightarrow> nat" where
+definition total_max_reg :: "transition \<Rightarrow> nat" where
   "total_max_reg t = (case max_reg t of None \<Rightarrow> 0 | Some a \<Rightarrow> a)"
 
-definition enumerate_ints :: "('a::aexp_value) transition \<Rightarrow> int set" where
+definition enumerate_ints :: "transition \<Rightarrow> int set" where
   "enumerate_ints t = (\<Union> (set (map enumerate_gexp_ints (Guards t)))) \<union>
                       (\<Union> (set (map enumerate_aexp_ints (Outputs t)))) \<union>
                       (\<Union> (set (map (\<lambda>(_, u). enumerate_aexp_ints u) (Updates t)))) \<union>
-                      (\<Union> (set (map (\<lambda>(r, _). {int r}) (Updates t))))"
+                      (\<Union> (set (map (\<lambda>(r, _). enumerate_aexp_ints (V (R r))) (Updates t))))"
 
-definition valid_transition :: "'a transition \<Rightarrow> bool" where
+definition valid_transition :: "transition \<Rightarrow> bool" where
   "valid_transition t = (\<forall>i \<in> enumerate_inputs t. i < Arity t)"
 
-definition can_take :: "nat \<Rightarrow> (vname,'a::aexp_value) gexp list \<Rightarrow> 'a inputs \<Rightarrow> 'a registers \<Rightarrow> bool" where
+definition can_take :: "nat \<Rightarrow> vname gexp list \<Rightarrow> inputs \<Rightarrow> registers \<Rightarrow> bool" where
   "can_take a g i r = (length i = a \<and> apply_guards g (join_ir i r))"
 
 lemma can_take_empty [simp]: "length i = a \<Longrightarrow> can_take a [] i c"
@@ -101,7 +99,7 @@ lemma cant_take_if:
    \<not> can_take_transition t i r"
   using apply_guards_cons apply_guards_rearrange can_take_def can_take_transition_def by blast
 
-definition apply_outputs :: "'a output_function list \<Rightarrow> ('a::aexp_value) datastate \<Rightarrow> 'a outputs" where
+definition apply_outputs :: "'a aexp list \<Rightarrow> 'a datastate \<Rightarrow> value option list" where
   "apply_outputs p s = map (\<lambda>p. aval p s) p"
 
 abbreviation "evaluate_outputs t i r \<equiv> apply_outputs (Outputs t) (join_ir i r)"
@@ -110,7 +108,7 @@ lemma apply_outputs_nth:
   "i < length p \<Longrightarrow> apply_outputs p s ! i = aval (p ! i) s"
   by (simp add: apply_outputs_def)
 
-lemmas apply_outputs = datastate apply_outputs_def plus_value_def minus_value_def times_value_def
+lemmas apply_outputs = datastate apply_outputs_def value_plus_def value_minus_def value_times_def
 
 lemma apply_outputs_empty [simp]: "apply_outputs [] s = []"
   by (simp add: apply_outputs_def)
@@ -132,13 +130,13 @@ lemma apply_outputs_unupdated: assumes "ia \<noteq> r"
     shows "apply_outputs P j ! ia = apply_outputs (list_update P r v)j ! ia"
   by (metis apply_outputs_nth assms(1) assms(2) length_list_update nth_list_update_neq)
 
-definition apply_updates :: "'a update_function list \<Rightarrow> ('a::aexp_value) datastate \<Rightarrow> 'a registers \<Rightarrow> 'a registers" where
+definition apply_updates :: "update_function list \<Rightarrow> vname datastate \<Rightarrow> registers \<Rightarrow> registers" where
   "apply_updates u old = fold (\<lambda>h r. r(fst h $:= aval (snd h) old)) u"
 
 abbreviation "evaluate_updates t i r \<equiv> apply_updates (Updates t) (join_ir i r) r"
 
 lemma apply_updates_cons: "ra \<noteq> r \<Longrightarrow>
-       apply_updates u s c $ ra = apply_updates ((r, a) # u) s c $ ra"
+       apply_updates u (join_ir ia c) c $ ra = apply_updates ((r, a) # u) (join_ir ia c) c $ ra"
 proof(induct u rule: rev_induct)
   case Nil
   then show ?case
@@ -157,32 +155,28 @@ lemma update_twice:
 
 lemma r_not_updated_stays_the_same:
   "r \<notin> fst ` set U \<Longrightarrow> apply_updates U c d $ r = d $ r"
-proof (induct U)
-  case Nil
-  then show ?case
-    by (simp add: apply_updates_def)
-next
-  case (Cons a U)
-  then show ?case
-    by (cases a, simp add: apply_updates_cons[symmetric])
-qed
+  using apply_updates_def
+  by (induct U rule: rev_induct, auto)
 
-definition rename_regs :: "(nat \<Rightarrow> nat) \<Rightarrow> 'a transition \<Rightarrow> 'a transition" where
+definition rename_regs :: "(nat \<Rightarrow> nat) \<Rightarrow> transition \<Rightarrow> transition" where
   "rename_regs f t = t\<lparr>
       Guards  := map (GExp.rename_regs f) (Guards t),
       Outputs := map (AExp.rename_regs f) (Outputs t),
       Updates := map (\<lambda>(r, u). (f r, AExp.rename_regs f u)) (Updates t)
     \<rparr>"
 
-definition eq_upto_rename_strong :: "'a transition \<Rightarrow> 'a transition \<Rightarrow> bool" where
+definition eq_upto_rename_strong :: "transition \<Rightarrow> transition \<Rightarrow> bool" where
   "eq_upto_rename_strong t1 t2 = (\<exists>f. bij f \<and> rename_regs f t1 = t2)"
 
-inductive eq_upto_rename :: "('a::aexp_value) transition \<Rightarrow> 'a transition \<Rightarrow> bool" where
+inductive eq_upto_rename :: "transition \<Rightarrow> transition \<Rightarrow> bool" where
   "Label t1 = Label t2 \<Longrightarrow>
    Arity t2 = Arity t2 \<Longrightarrow>
    apply_guards (map (GExp.rename_regs f) (Guards t1)) = apply_guards (Guards t2) \<Longrightarrow>
+
    apply_outputs (map (AExp.rename_regs f) (Outputs t1)) = apply_outputs (Outputs t2) \<Longrightarrow>
+
    apply_updates (map (\<lambda>(r, u). (f r, AExp.rename_regs f u)) (Updates t1)) = apply_updates (Updates t2) \<Longrightarrow>
+
    eq_upto_rename t1 t2"
 
 end
